start again

RowPredicates/Basic.lean
@@ -1,246 +1,199 @@
---------------
--- TODOs
---------------
+ module
 
-inductive Label : Type where
-  | label : String -> Label
-  -- LVar : String/Number -> Label
+public import RowPredicates.Label
 
-deriving instance BEq, DecidableEq for Label
+@[expose] public section
 
--- Idea: redefine Row as a finset of fields.
--- Or just as a dictionary.
--- Would need to map fields to their labels to compare label sets
+namespace Rope
+
+open Label
+
+-- inductive LabelTerm where
+-- | Concrete : String -> LabelTerm
+-- | LVar : String -> LabelTerm
+
+-- Start off by just capturing the abstract term syntax
+-- without mutual recursion
+
+inductive Term : Type where
+  | RVar : (name : String) -> Term
+  | TVar : (name : String) -> Term
+  | TFun : Term -> Term -> Term
+  | Field : Label -> Term -> Term
+  | Row : List Term -> Term
+  | Singleton : Label -> Term
+  | Pi : Term -> Term
+  | Sigma : Term -> Term
+  -- leaving off type-level functions now to keep it simple
+  -- | TApp
+  -- | TLam
+
+inductive Kind : Type where
+  | KTy : Kind
+  | KRow : Kind
+
+-- Assert that all fields in the field list have a term which satisfies the given propositional predicate
+inductive AllFields : (Pred: Term -> Prop) -> List Term -> Prop where
+  | Nil : (AllFields Pred [])
+  | Cons : Pred t -> AllFields Pred fields -> (AllFields Pred ((Term.Field l t)::fields))
+
+-- Well-Kindedness Judgement
+inductive Term.WK : Term -> Kind -> Prop where
+  | RVar : (name : String) -> WK (.RVar name) KRow
+  | TVar : (name : String) -> WK (.TVar name) KTy
+  | TFun : (Term.WK arg Ty) -> (Term.WK ret Ty) -> (Term.WK (TFun arg ret) Ty)
+  -- | Field : (Term.WK t) -> Term
+  | Row : (fields: List Term) -> (AllFields (λ t => Term.WK t .KTy) fields) -> (Term.WK (Row fields) KRow)
+
+inductive PredTerm : Type where
+  | Leq : Term -> Term -> PredTerm
+  | Eq : Term -> Term -> PredTerm
+  -- Garrett-style 3-place concatenation predicate
+  -- x + y ~ z
+  | Concat : Term -> Term -> Term -> PredTerm
+
+inductive PredTerm.WK : PredTerm -> Prop where
+  | Leq : Term.WK x KRow -> Term.WK y KRow -> PredTerm.WK (PredTerm.Leq x y)
+  | Eq : Term.WK x KRow -> Term.WK y KRow -> Term.WK y KRow -> PredTerm.WK (PredTerm.Concat x y z)
+  | Concat : Term.WK x KRow -> Term.WK y KRow -> Term.WK y KRow -> PredTerm.WK (PredTerm.Concat x y z)
+
 mutual
--- Pre-Row?
-inductive Row : Type where
-  | empty : Row                                               -- (Identity for Concat)
-  | extend : Row -> Label -> Ty -> Row
-  -- | concat : Row -> Row -> Ty
-  -- | RVar : String -> Row
-  -- Complement/RowMinus : x: Row -> y: Row -> Disjoint x y -> Row
+inductive PreRow : Type where
+  | empty : PreRow -- (Identity for Concat)
+  | rVar : String -> PreRow
+  | extend : PreRow -> Label -> PreTy -> PreRow
 
-inductive Ty : Type where
-  | Pi : Row -> Ty
-  | Sigma : Row -> Ty
-  | TVar : String -> Ty
-  -- | TFun : Ty -> Ty
-  -- | Exact : Label -> Ty
+inductive PreTy : Type where
+  | TVar (name : String) : PreTy
+  | TFun (arg: PreTy) (ret: PreTy) : PreTy
+  | Singleton : Label -> PreTy
+  | Pi : PreRow -> PreTy
+  | Sigma : PreRow -> PreTy
 end
 
+inductive PreRow.lack : PreRow -> (Label) -> Prop where
+  | empty : PreRow.lack .empty l
+  | rVar : l ≠ l -> PreRow.lack (PreRow.rVar s) l
+  | extend : PreRow.lack r l -> l ≠ l' -> PreRow.lack (extend r l' t) l
 
--- declare_syntax_cat label
--- syntax "{" ident "}" : label
+inductive PreRow.disjoint : PreRow -> PreRow -> Prop where
+  | refl : disjoint .empty .empty
+  | extend : disjoint r1 r2 -> l1 ≠ l2 -> r1.lack l2 -> r2.lack l1 -> disjoint (.extend r1' l1 t1) (.extend r2' l2 t2)
 
--- #check_failure *(* (Label.Label "hello") @@ (@ "l") *)*
+inductive PreRow.unique_labels : PreRow -> Prop where
+  | empty : unique_labels .empty
+  | rVar : unique_labels (.rVar s)
+  | extend : unique_labels r -> lack r l -> unique_labels (extend r l t)
 
--- def l : Label := hello
+-- Row is concrete (Has explicit labels and is not a variable)
+inductive PreRow.concrete : PreRow -> Prop where
+  | empty : concrete .empty
+  | extend : concrete r -> Label.concrete l -> lack r l -> concrete (extend r l t)
 
--- declare_syntax_cat labeledField
--- syntax label " := " term : labeledField
+-- Interdefined Well-formedness rules for PreRow and PreTy
+mutual 
+inductive Row.WF : (inner: PreRow) -> Prop where
+  | empty : Row.WF .empty
+  | rVar : Row.WF (.rVar s)
+  | extend : Row.WF r -> PreRow.unique_labels r -> r.lack l -> (Ty.WF t) -> Row.WF (.extend r l t)
 
+inductive Ty.WF : (inner: PreTy) -> Prop where
+  | TVar : Ty.WF (.TVar s)
+  | TFun : Ty.WF arg -> Ty.WF ret -> Ty.WF (.TFun (arg: PreTy) (ret: PreTy))
+  | Singleton : Ty.WF (.Singleton l)
+  | Pi : PreRow -> Row.WF r -> Ty.WF (.Pi r)
+  | Sigma : PreRow -> Row.WF r -> Ty.WF (.Sigma r)
+end
 
+open PreRow Row.WF
 
+-- I'll have to see how it feels to induct over these types?
+inductive Row : Type where
+| mk (inner : PreRow)
+     (wf : Row.WF inner) : Row
+-- Row must be implemented on top of PreRow and bundle well-formedness invariant
 
-def field (s: String) (t: Ty) : Row :=
-  .extend .empty (.label s) t
+inductive Ty : Type where
+| mk (inner : PreTy)
+     (wf : Ty.WF inner) : Ty
 
-notation "*" l => Label.label l
-
--- -- TODO(mctano) : Improve this notation
--- maybe make it use concat, once defined, to enforce disjointness constraints,
 notation "{}" => Row.empty
-notation l " : " t ", " tail => Row.extend tail (Label.label l) t
+notation l " : " t ", " tail => Row.extend tail l t
 notation "@@" t => Ty.TVar t
 
--- #check ("hello" : @@"goodbye", "2" : @@"hello", "3rd" : @@"oopsie", {})
+def Row.inner : Row -> PreRow
+  | (.mk inner _) => inner
+
+def Row.wf : (r : Row) -> Row.WF r.inner
+  | (.mk _ wf) => wf
 
 
 
-inductive Lacks : Row -> Label -> Prop where
-  | empty : {l : Label} -> Lacks .empty l
-  | extend : (r: Row) -> (l : Label) -> (l' : Label) -> (Lacks r l) -> l ≠ l' -> {t : Ty} -> (Lacks (.extend r l' t) l)
+def Row.unique_labels : Row -> Prop
+  | (.mk inner _) => inner.unique_labels
 
-inductive In : Label -> Row ->  Prop where
-  | label l {t} r' : In l (Row.extend r' l t)
-  | ind l {t} r' l' : In l r' -> In l (Row.extend r' l' t)
+-- A row lacks a label iff the inner (well-formed) pre-row lacks that label
+def Row.lack : Row -> Label -> Prop
+  | (.mk inner _), l => inner.lack l
 
+def Row.disjoint : Row -> Row -> Prop
+  | (.mk innerL _), (.mk innerR _) => innerL.disjoint innerR
 
-def decide_in (l : Label) (r : Row) : (In l r) ∨ (Lacks r l) :=
+def Row.concrete : Row -> Prop
+  | (.mk inner _) => inner.concrete
+
+theorem PreRow.unique_labels_lack_extend : PreRow.unique_labels (.extend r l t) -> PreRow.lack r l := by
+  intro h
+  cases h
+  assumption
+
+theorem PreRow.unique_labels_extend {pr : PreRow} {l t} : PreRow.unique_labels (.extend pr l t) -> PreRow.unique_labels pr := by
+  cases pr <;> intro h
+  apply unique_labels.empty
+  apply unique_labels.rVar
+  cases h <;> assumption
+
+theorem row_unique_labels : ∀ (r : Row), Row.concrete r -> Row.unique_labels r
+  | (.mk inner wf) => by
+    intro h
+    cases h <;> simp [Row.unique_labels] <;> cases wf <;> constructor <;> assumption
+
+-- This should (maybe?) bundle evidence eventually
+inductive Pred : Type where
+  | Leq (x: Row) (y: Row) : Pred
+  | Concat (x: Row) (y: Row) (z: Row) :Pred
+  | Eq (x: Row) (y: Row) : Pred
+
+def PreRow.typeAt (r: PreRow) (l: Label) : Option PreTy :=
   match r with
-  | .empty => .inr .empty
-  | .extend r' l' t' => 
-                        dite (l = l')
-                          (λ h_eq => .inl (by rw [<- h_eq]; exact In.label l r'))
-                          (λ h_neq => match decide_in l r' with
-                                      | .inl h => Or.inl (In.ind l r' l' h)
-                                      | .inr h => Or.inr (Lacks.extend _ _ _ h h_neq))
+    | .empty => .none
+    -- 
+    | .rVar _ => .none
+    | .extend r' l' t =>
+      if (l = l')
+      then .some t
+      else typeAt r' l
 
-inductive Disjoint : Row -> Row -> Prop where
-  | empty : Disjoint .empty .empty
-  | extendL : (r1 : Row) -> (r2 : Row) -> (l :Label) -> {t : Ty} -> Disjoint r1 r2
-      -> Lacks r2 l -> Disjoint (.extend r1 l t) r2
-  | extendR : (r1 : Row) -> (r2 : Row) -> (l :Label) -> {t : Ty} -> Disjoint r1 r2
-    -> Lacks r1 l -> Disjoint r1 (.extend r2 l t)
+-- This should propagate the well-formedness invariant of the returned type
+-- def typeAt (r: Row) (l: Label) : Option Ty :=
+--   match r.inner.typeAt l with
+--   | .some t => t
 
-theorem disjoint_symm {r1 r2 : Row} (h: Disjoint r1 r2) : Disjoint r2 r1 :=
-  match h with
-  | .empty => .empty
-  | .extendL r1 r2 l h_disj h_lack1 => by apply Disjoint.extendR _ _ _ (disjoint_symm h_disj) h_lack1
-  | .extendR r1 r2 l h_disj h_lack1  => by apply Disjoint.extendL _ _ _ (disjoint_symm h_disj) h_lack1
+def PreRow.contained_in (r1 r2: PreRow) : Prop :=
+  forall (l1 : Label), (typeAt r1 l1) = (typeAt r2 l1)
 
-theorem emptyRowDisjointL {r: Row} :  Disjoint .empty r :=
-  match r with
-  | .empty => .empty
-  | .extend r' _ _ => Disjoint.extendR .empty r' _ emptyRowDisjointL Lacks.empty
-
-theorem emptyRowDisjointR {r: Row} : Disjoint r .empty := by
-  apply disjoint_symm
-  exact emptyRowDisjointL
-
-inductive WellFormed : Row -> Prop where
-  | empty : WellFormed .empty
-  | extend : (r: Row) -> (l: Label) -> (t: Ty) -> WellFormed r -> Lacks r l -> (WellFormed (.extend r l t))
-
-theorem lacks_extend_lacks {r: Row} {l1 l2: Label} {t: Ty} (h_lack: Lacks (r.extend l2 t) l1) : Lacks r l1 :=
-  match h_lack with
-  | .extend _ _ _ h _ => h
-
-theorem lacks_implies_neq' {r1 : Row} {l1 l2 : Label} {t1: Ty} (h: Lacks (r1.extend l1 t1) l2): l2 ≠ l1 :=
-  match h with
-  | .extend _  _ _ _ h_neq => (λ h_eq => h_neq h_eq)
-
-theorem lacks_implies_neq {r1 : Row} {l1 l2 : Label} {t1: Ty} (h: Lacks (r1.extend l1 t1) l2): l1 ≠ l2 :=
-  by symm
-     apply lacks_implies_neq' h
-
-
-theorem disjoint_extend_implies_neq {r1 r2 : Row} {l1 l2 : Label} {t1 t2: Ty} (h : Disjoint (r1.extend l1 t1) (r2.extend l2 t2)): l1 ≠ l2 :=
-  match h with
-  | .extendL _ _ _ _ hl => lacks_implies_neq' hl
-  | .extendR _ _ _ _ hl => lacks_implies_neq hl
-
-theorem disjoint_extend_injectL {r1 r2 : Row} {l1 t1} (h : Disjoint (r1.extend l1 t1) r2) : Disjoint r1 r2 :=
-  match h with
-  | .extendL _ _ _ h' _ => h'
-  | .extendR _ r2' _ h' h'' => by apply Disjoint.extendR _ _ _ (disjoint_extend_injectL h') (lacks_extend_lacks h'')
-
-theorem disjoint_extend_injectR {r1 r2 : Row} {l1 t1} (h : Disjoint r1 (r2.extend l1 t1)) : Disjoint r1 r2 :=
-  match h with
-  | .extendL r1' _ _ h' h'' => by apply Disjoint.extendL _ _ _ (disjoint_extend_injectR h') (lacks_extend_lacks h'')
-  | .extendR _ _ _ h' _ => h'
-
-theorem disjoint_extend_inject (r1 r2 : Row) {l1 l2 : Label} {t1 t2 : Ty} (h : Disjoint (r1.extend l1 t1) (r2.extend l2 t2)) : Disjoint r1 r2 :=
-  disjoint_extend_injectL (disjoint_extend_injectR h)
-
-  -- match h with
-  -- | .empty => .empty
-  -- | .extendL r1' r2' l' _ h' h'' => by apply Lacks.extend _ _ _
-  --                                   apply
-  --                                   sorry
-  --                                   sorry
-  -- | .extendR _ _ _ _ e _ => sorry
-  -- | .empty => sorry
-
--- def concat (r1 : Row) (r2 : Row) (h1: WellFormed r1) (h2: WellFormed r2) (h_disj: Disjoint r1 r2) : Row :=
---   match r1 with
---     | .empty => r2
---     | r1 => match r2 with
---             | .empty => r1
---             | .extend r2' l t =>
---               let h1' := by
---                 apply WellFormed.extend _  _  _ h1
-                
-                
-                
---                 sorry    
---               let h2' := by sorry
---               let h3' := by sorry
---               concat (.extend r1 l t) r2' h1' h2' h3'
-  -- | .empty .empty => .empty
-
-
--- This is missing the commutativity of row entries.
--- Look at how set inclusion, subset, and equality are defined.
-inductive ContainedIn : Row -> Row -> Prop where
-  | refl : {r: Row} -> ContainedIn r r
-  | extend : (r1: Row) -> (r2: Row) -> (l : Label) -> (t : Ty) -> ContainedIn r1 r2 -> ContainedIn r1 (.extend r2 l t)
-
-theorem contain_extend {r1 r2 : Row} {l : Label} {t : Ty} (h: ContainedIn (.extend r1 l t) r2) : ContainedIn r1 r2 :=
-  match h with
-  | .refl => ContainedIn.extend _ _ _ _ .refl
-  | .extend _ _ _ _ h' => ContainedIn.extend _ _ _ _ (contain_extend h')
-                                 
-
-theorem contain_trans {r1 r2 r3 : Row} (h1: ContainedIn r1 r2) (h2: ContainedIn r2 r3) : ContainedIn r1 r3 := 
-  match h1 with
-  | .refl => h2
-  | .extend _ r' l t h' => contain_trans h' (contain_extend h2)
-
-theorem empty_contain_trivial {r: Row} : ContainedIn .empty r :=
-  match r with
-  | .empty => .refl
-  | .extend _ _ _ => contain_trans empty_contain_trivial (contain_extend .refl)
-
-theorem contain_empty_refl_only {r : Row} (h: ContainedIn r .empty) : r = .empty := by
-  cases r
-  case _ => eq_refl
-  case _ => contradiction
-
--- inductive Row.Subset : Row -> Row -> Prop where
-
-
-inductive Row.Equiv : Row -> Row -> Prop where
-  | refl {r : Row} : Equiv r r
-  | extend (r1 r2: Row) l t : Equiv r1 r2 -> Equiv (extend r1 l t) (extend r2 l t)
-
-
-
--- This can't be defined until I define equality for rows.
--- I probably also need to figure out how to encode the disjointness constraint for extending rows.
--- theorem contain_antisymm {r1 r2: Row} (h1 : ContainedIn r1 r2) (h2: ContainedIn r2 r1) : r1 = r2 := by
---   induction r2 generalizing r1
---   case _ => apply contain_empty_refl_only h1
---   case _ r' t h1' ih => sorry
-
-
-
-
--- define Predicate (TBD which should be atomic)
-  -- ContainedIn : Row -> Row -> Predicate
-  -- Equal : Row -> Row -> Predicate
-  -- LabelOf : Label -> Row -> Predicate                                               -- I want this as a way to assert field presence/absence without introducing a type variable.
-  -- Disjoint : Row -> Row -> Predicate
-  -- Not : Predicate -> Predicate (alternative to having a negative judgement form.)
+def Row.contained_in (a b : Row) : Prop :=
+  a.inner.contained_in b.inner
   
-  -- Derived:
-  -- NotLabelOf : Label -> Row -> Predicate                                            -- defined as (Not . LabelOf)
+instance : LE Row where
+  le := Row.contained_in
 
+def Row.contained_in_trans {r1 r2 r3 : Row} (h_1_2: contained_in r1 r2) (h_2_3: contained_in r2 r3): contained_in r1 r3 := by
+  intro l;
+  rw [h_1_2, h_2_3]
 
-
--- define Kind system
-  -- R[k]
-  -- Type
-  -- Label
-  -- KFun : Kind -> Kind -> Kind
-
--- define Predicate Derivation Rules
-  -- Do we want a negative judgement form? Could just make predicates negatable.
-  -- May need to divide these into terminating/non-terminating rulesets.
-
-
---------------
--- TODOs
---------------
-
--- relate Row Predicate Calculus to Monoids
--- Determine equivalent logical system under Curry-Howard-Correspondence.
--- find the simplest system that can express everything we need.
--- see what proofs that gets us for free.
--- prove properties of ruleset:
-  -- Soundness
-  -- Prove that the calculus is undecidable?
-  -- Give a best-effort Decision Procedure (DP).
-    -- Could use bounded recursion to run a not-necessarily terminating process for a finite time.
-  -- Prove Soundness of DP.
-  -- Prove something about how the DP approaches or approximates Completeness, or that it works under certain conditions.
+instance : Std.IsPreorder Row where
+  le_refl := λ x =>
+    by intro l
+       rfl
+  le_trans := λ _ _ _ => Row.contained_in_trans
