RowPredicates.lean
@@ -1,3 +1,5 @@
 -- This module serves as the root of the `RowPredicates` library.
 -- Import modules here that should be built as part of the library.
 import RowPredicates.Basic
+import RowPredicates.Label
+import RowPredicates.Row1
