RowPredicates/Label.lean
@@ -1,0 +1,30 @@
+module
+
+
+@[expose] public section
+
+namespace Label
+
+inductive Label : Type where
+  | label (s : String)  : Label
+  | LVar (name: String) : Label
+
+inductive Label.concrete : Label -> Prop where
+ | literal : Label.concrete (.label s)
+
+deriving instance BEq, ReflBEq, DecidableEq, Hashable, Ord for Label
+
+-- This actually only makes sense for concrete labels
+-- I'm still not totally sure whether LVar should be a case of Label or of Term
+-- We do need boolean equality for labels, but i guess in the literal case it would
+-- actually be easy enough to match on and compare the string contents
+-- instance : BEq Label where
+--   beq := λ (.label a) (.label b) => a == b
+
+-- instance : LawfulBEq Label where
+--   rfl := instBEqLabel.rfl
+--   eq_of_beq := λ {a b} h => by
+--     cases a
+--     cases b
+--     simp [(·==·)] at h
+--     rw [h]
